not in a tidy order yet but anyway works...

ETCSFin.sml
@@ -1,32 +1,3 @@
-val p31_ex = prove_store("p31_ex",
-e0
-(rpt strip_tac >> qexists_tac ‘p1(A,B * C)’ >> rw[])
-(form_goal
- “!A B C. ?p31: A * B * C ->A. p1(A,B * C) = p31”));
-
-val p31_def = p31_ex |> spec_all |> eqT_intro
-                     |> iffRL |> ex2fsym "p31" ["A","B","C"]
-                     |> C mp (trueI []) |> gen_all
-
-val p32_ex = prove_store("p32_ex",
-e0
-(rpt strip_tac >> qexists_tac ‘p1(B,C) o p2(A,B * C)’ >> rw[])
-(form_goal
- “!A B C. ?p32: A * B * C ->B.p1(B,C) o p2(A,B * C) = p32”));
-
-val p32_def = p32_ex |> spec_all |> eqT_intro
-                     |> iffRL |> ex2fsym "p32" ["A","B","C"]
-                     |> C mp (trueI []) |> gen_all
-
-val p33_ex = prove_store("p33_ex",
-e0
-(rpt strip_tac >> qexists_tac ‘p2(B,C) o p2(A,B * C)’ >> rw[])
-(form_goal
- “!A B C. ?p33: A * B * C ->C.p2(B,C) o p2(A,B * C) = p33”));
-
-val p33_def = p33_ex |> spec_all |> eqT_intro
-                     |> iffRL |> ex2fsym "p33" ["A","B","C"]
-                     |> C mp (trueI []) |> gen_all
 
                     
 
@@ -100,26 +71,6 @@ val Del_def =
 
 
 
-val p31_of_Pa = prove_store("p31_of_Pa",
-                            e0
-                                (rpt strip_tac >> rw[GSYM p31_def,p1_of_Pa] )
-                                (form_goal
-                                     “!A B C X a:X-> A bc: X-> B * C. p31(A,B,C) o Pa(a, bc) = a”));
-
-
-val p32_of_Pa = prove_store("p32_of_Pa",
-e0
-(rpt strip_tac >> rw[GSYM p32_def,o_assoc,p12_of_Pa] )
-(form_goal
-“!A B C X a:X-> A b: X-> B c: X-> C. p32(A,B,C) o Pa(a, Pa(b,c)) = b”));
-
-
-val p33_of_Pa = prove_store("p33_of_Pa",
-e0
-(rpt strip_tac >> rw[GSYM p33_def,o_assoc,p2_of_Pa] )
-(form_goal
-“!A B C X a:X-> A b: X-> B c: X-> C. p33(A,B,C) o Pa(a, Pa(b,c)) = c”));
-
 val Ins_property = prove_store("Ins_property",
 e0
 (rpt strip_tac >> rw[GSYM Ins_def,GSYM Insert_def,Ev_of_Tp] >> 
@@ -145,87 +96,6 @@ e0
   (Ev(X,1+1) o Pa(x,s0) = TRUE & ~(x = x0))”));
 
 
-
-
-val Pa3_ex = prove_store("Pa3_ex",
-e0
-(rpt strip_tac >> qexists_tac ‘Pa(f,Pa(g,h))’ >> rw[])
-(form_goal
- “!A B C X f:X->A g:X ->B h:X->C. ?Pa3.
- Pa(f,Pa(g,h)) = Pa3 
-”));
-
-
-val Pa3_def = Pa3_ex |> spec_all |> eqT_intro
-              |> iffRL |> ex2fsym "Pa3" ["f","g","h"]
-              |> C mp (trueI []) |> gen_all
-
-val Pa4_ex = prove_store("Pa4_ex",
-e0
-(rpt strip_tac >> qexists_tac ‘Pa(f,Pa(g,Pa(h,j)))’ >> rw[])
-(form_goal
- “!A B C D X f:X->A g:X ->B h:X->C j:X->D. ?Pa4.
- Pa(f,Pa(g,Pa(h,j))) = Pa4
-”));
-
-val Pa4_def = Pa4_ex |> spec_all |> eqT_intro
-              |> iffRL |> ex2fsym "Pa4" ["f","g","h","j"]
-              |> C mp (trueI []) |> gen_all
-
-val p41_ex = prove_store("p41_ex",
-e0
-(rpt strip_tac >> qexists_tac ‘p1(A, B * C * D)’ >> rw[])
-(form_goal 
- “!A B C D. ?p41. p1(A,B * C * D) = p41”));
-
-val p41_def = p41_ex |> spec_all |> eqT_intro
-              |> iffRL |> ex2fsym "p41" ["A","B","C","D"]
-              |> C mp (trueI []) |> gen_all
-
-val p42_ex = prove_store("p42_ex",
-e0
-(rpt strip_tac >> qexists_tac ‘p1(B, C * D) o p2(A,B * C * D)’ >> rw[])
-(form_goal 
- “!A B C D. ?p42. p1(B, C * D) o p2(A,B * C * D) = p42”));
-
-
-val p42_def = p42_ex |> spec_all |> eqT_intro
-              |> iffRL |> ex2fsym "p42" ["A","B","C","D"]
-              |> C mp (trueI []) |> gen_all
-
-
-val p43_ex = prove_store("p43_ex",
-e0
-(rpt strip_tac >> qexists_tac ‘p1(C,D) o p2(B, C * D) o p2(A,B * C * D)’ >> rw[])
-(form_goal 
- “!A B C D. ?p43. p1(C,D) o p2(B, C * D) o p2(A,B * C * D) = p43”));
-
-
-val p43_def = p43_ex |> spec_all |> eqT_intro
-              |> iffRL |> ex2fsym "p43" ["A","B","C","D"]
-              |> C mp (trueI []) |> gen_all
-
-
-val p44_ex = prove_store("p44_ex",
-e0
-(rpt strip_tac >> qexists_tac ‘p2(C,D) o p2(B, C * D) o p2(A,B * C * D)’ >> rw[])
-(form_goal 
- “!A B C D. ?p44. p2(C,D) o p2(B, C * D) o p2(A,B * C * D) = p44”));
-
-
-val p44_def = p44_ex |> spec_all |> eqT_intro
-                     |> iffRL |> ex2fsym "p44" ["A","B","C","D"]
-                     |> C mp (trueI []) |> gen_all
-
-fun mk_o a1 a2 = mk_fun "o" [a1,a2]
-
-val CONJ = mk_fun "CONJ" []
-
-fun Pa f g = mk_fun "Pa" [f,g]
-
-fun Ex X = mk_fun "Ex" [X]
-
-fun Tp f = mk_fun "Tp" [f]
 
 
 
@@ -269,7 +139,7 @@ rastt $ q2str
                     p32(X,Exp(X,1+1),Exp(Exp(X,1+1),1+1))),
                 p33(X,Exp(X,1+1),Exp(Exp(X,1+1),1+1))))’
 
-val IMP = mk_fun "IMP" []
+
 
 val longpred0 = 
 mk_o (rastt "All(Exp(X,1+1))") $ Tp (mk_o IMP (Pa longpred_ant longpred_conc))
@@ -331,7 +201,7 @@ mk_o (mk_o (rastt "Ev(Exp(X,1+1),1+1)")
 (Pa (rastt "p1(Exp(X,1+1),1)") (mk_o finites (rastt "p2(Exp(X,1+1),1)")))) (rastt "Pa(id(Exp(X,1+1)),To1(Exp(X,1+1)))")
 
 
-val two = rastt "1+1";
+
 
 val isFinite_ex = prove_store("isFinite_ex",
 e0
@@ -348,28 +218,6 @@ isFinite_ex |> spec_all |> eqT_intro
             |> iffRL |> ex2fsym "isFinite" ["X"] 
             |> C mp (trueI []) |> gen_all;
 
-
-
-val p31_of_Pa3 = proved_th $
-e0
-(rpt strip_tac >> rw[GSYM Pa3_def,GSYM p31_def,p1_of_Pa])
-(form_goal
-“!A B C X f:X->A g:X->B h:X->C. p31(A,B,C) o Pa3(f,g,h) = f”)
-
-
-
-val p32_of_Pa3 = proved_th $
-e0
-(rpt strip_tac >> rw[GSYM Pa3_def,GSYM p32_def,p12_of_Pa,o_assoc])
-(form_goal
-“!A B C X f:X->A g:X->B h:X->C. p32(A,B,C) o Pa3(f,g,h) = g”)
-
-
-val p33_of_Pa3 = prove_store("p33_of_Pa3",
-e0
-(rpt strip_tac >> rw[GSYM Pa3_def,GSYM p33_def,p2_of_Pa,o_assoc])
-(form_goal
-“!A B C X f:X->A g:X->B h:X->C. p33(A,B,C) o Pa3(f,g,h) = h”));
 
 val isFinite_property = prove_store("isFinite_property",
 e0
@@ -397,27 +245,6 @@ rw[GSYM Mem_def] >> once_rw[one_to_one_id] >> rw[idR]
 
 
 
-val Ev_of_Tp_el' = prove_store("Ev_of_Tp_el'",
-e0
-(rpt strip_tac >> 
- qby_tac ‘Tp(f) = Tp(f) o id(P)’ >-- rw[idR] >>
- once_arw[] >> rw[Ev_of_Tp_el])
-(form_goal
-“!A B P f:A * P -> B  a:P -> A.
-Ev(A, B) o Pa(a, Tp(f)) = f o Pa(a, id(P))”));
-
-
-val Ev_of_el = prove_store("Ev_of_el",
-e0
-(rpt strip_tac >>
- qby_tac 
- ‘f = Tp1(Tp0(f))’ >-- rw[Tp1_Tp0_inv] >> once_arw[] >>
- rw[GSYM Tp1_def,Ev_of_Tp_el'] >> rw[Tp1_def,Tp1_Tp0_inv] >>
- rw[o_assoc,p1_of_Pa,idR])
-(form_goal
- “!A B f:1->Exp(A,B) a:1->A.
-  Ev(A,B) o Pa(a,f) = Tp0(f) o a”));
-
 
 val isFinite_property1 =prove_store("isFinite_property1",
 e0
@@ -436,7 +263,7 @@ e0
  P o a = TRUE
  ”));
 
-fun Po A B = mk_fun "*" [A,B]
+
 
 val FINITE_def = new_ax 
 “!X. FINITE(X) <=> isFinite(X) o Tp1(True(X)) =TRUE”
@@ -467,7 +294,7 @@ e0
 
 
 
-
+(*
 val p41_ex = prove_store("p41_ex",
 e0
 (rpt strip_tac >> qexists_tac ‘p1(A, B * C * D)’ >> rw[])
@@ -513,65 +340,10 @@ val p44_def = p44_ex |> spec_all |> eqT_intro
               |> iffRL |> ex2fsym "p44" ["A","B","C","D"]
               |> C mp (trueI []) |> gen_all
 
+*)
 
 
-
-
-val p41_of_Pa4 = prove_store("p41_of_Pa4",
-e0
-(rpt strip_tac >> rw[GSYM Pa4_def,GSYM p41_def,p12_of_Pa])
-(form_goal
-“!A B C D X f:X->A g:X->B h:X->C k:X->D.
- p41(A,B,C,D) o Pa4(f,g,h,k) = f”));
-
-val p42_of_Pa4 = prove_store("p42_of_Pa4",
-e0
-(rpt strip_tac >> rw[GSYM Pa4_def,GSYM p42_def,p12_of_Pa,o_assoc])
-(form_goal
-“!A B C D X f:X->A g:X->B h:X->C k:X->D.
- p42(A,B,C,D) o Pa4(f,g,h,k) = g”));
-
-
-val p43_of_Pa4 = prove_store("p43_of_Pa4",
-e0
-(rpt strip_tac >> rw[GSYM Pa4_def,GSYM p43_def,p12_of_Pa,o_assoc])
-(form_goal
-“!A B C D X f:X->A g:X->B h:X->C k:X->D.
- p43(A,B,C,D) o Pa4(f,g,h,k) = h”));
-
-
-val p44_of_Pa4 = prove_store("p44_of_Pa4",
-e0
-(rpt strip_tac >> rw[GSYM Pa4_def,GSYM p44_def,p12_of_Pa,o_assoc])
-(form_goal
-“!A B C D X f:X->A g:X->B h:X->C k:X->D.
- p44(A,B,C,D) o Pa4(f,g,h,k) = k”));
-
-
-val Pa5_ex = prove_store("Pa5_ex",
-e0
-(rpt strip_tac >> qexists_tac ‘Pa(f,Pa(g,Pa(h,Pa(j,k))))’ >> rw[])
-(form_goal
- “!A B C D E X f:X->A g:X ->B h:X->C j:X->D k:X->E. ?Pa5.
- Pa(f,Pa(g,Pa(h,Pa(j,k)))) = Pa5
-”));
-
-val Pa5_def = Pa5_ex |> spec_all |> eqT_intro
-              |> iffRL |> ex2fsym "Pa5" ["f","g","h","j","k"]
-              |> C mp (trueI []) |> gen_all
-
-
-
-val p51_ex = prove_store("p51_ex",
-e0
-(rpt strip_tac >> qexists_tac ‘p1(A, B * C * D * E)’ >> rw[])
-(form_goal 
- “!A B C D E. ?p51. p1(A,B * C * D * E) = p51”));
-
-val p51_def = p51_ex |> spec_all |> eqT_intro
-              |> iffRL |> ex2fsym "p51" ["A","B","C","D","E"]
-              |> C mp (trueI []) |> gen_all
-
+(*
 val p42_ex = proved_th $
 e0
 (rpt strip_tac >> qexists_tac ‘p1(B, C * D) o p2(A,B * C * D)’ >> rw[])
@@ -596,28 +368,6 @@ val p43_def = p43_ex |> spec_all |> eqT_intro
               |> C mp (trueI []) |> gen_all
 
 
-val p55_ex = prove_store("p55_ex",
-e0
-(rpt strip_tac >> qexists_tac ‘p2(D,E) o p2(C, D * E) o p2(B,C * D * E) o p2(A,B * C * D * E)’ >> rw[])
-(form_goal 
- “!A B C D E. ?p55. p2(D,E) o p2(C, D * E) o p2(B,C * D * E) o p2(A,B * C * D * E) = p55”));
-
-
-val p55_def = p55_ex |> spec_all |> eqT_intro
-              |> iffRL |> ex2fsym "p55" ["A","B","C","D","E"]
-              |> C mp (trueI []) |> gen_all
-
-
-
-
-
-val p51_of_Pa5 = prove_store("p51_of_Pa5",
-e0
-(rpt strip_tac >> rw[GSYM Pa5_def,GSYM p51_def,p12_of_Pa])
-(form_goal
-“!A B C D E X f:X->A g:X->B h:X->C j:X->D k:X->E.
- p51(A,B,C,D,E) o Pa5(f,g,h,j,k) = f”));
-
 val p42_of_Pa4 = prove_store("p42_of_Pa4",
 e0
 (rpt strip_tac >> rw[GSYM Pa4_def,GSYM p42_def,p12_of_Pa,o_assoc])
@@ -632,33 +382,8 @@ e0
 (form_goal
 “!A B C D X f:X->A g:X->B h:X->C k:X->D.
  p43(A,B,C,D) o Pa4(f,g,h,k) = h”));
+*)
 
-
-val p55_of_Pa5 = prove_store("p55_of_Pa5",
-e0
-(rpt strip_tac >> rw[GSYM Pa5_def,GSYM p55_def,p12_of_Pa,o_assoc])
-(form_goal
-“!A B C D X f:X->A g:X->B h:X->C j:X->D k:X->E.
- p55(A,B,C,D,E) o Pa5(f,g,h,j,k) = k”));
-
-
-val Tp0_INJ = prove_store("Tp0_INJ",
-e0
-(rpt strip_tac >> dimp_tac >> strip_tac >-- 
- (once_rw[GSYM Tp1_Tp0_inv] >> arw[]) >> arw[])
-(form_goal
- “!A B f:1->Exp(A,B) g:1->Exp(A,B).
-  Tp0(f) = Tp0(g) <=> f = g”));
-
-val pred_ext = prove_store("pred_ext",
-e0
-(rpt strip_tac >> dimp_tac >> strip_tac (* 2 *) >-- 
- (cases_on “p1:1->1+1 = TRUE” >-- fs[] >>
- fs[TRUE2FALSE] >> fs[TRUE_ne_FALSE] >>
- fs[TRUE2FALSE]) >>
- arw[])
-(form_goal
-“!p1 p2. (p1 = TRUE <=> p2 = TRUE) <=> p1 = p2”));
 
 
 val ABSORPTION_RWT = prove_store("ABSORPTION_RWT",
@@ -765,7 +490,7 @@ e0
 (form_goal
  “!X x0 x:1->X.(~(x0 = x)) ==> !xs.Del(x,Ins(x0, xs)) = Ins(x0,Del(x,xs))”));
 
-fun Pow A = Exp A two
+
 
 
 val contain_empty_O = 
@@ -811,7 +536,7 @@ val sets_contain_pair = Tp1 longp
 
 val hasCard = mk_o (rastt "BIGINTER(Exp(X,1+1) * N)") sets_contain_pair
 
-fun Tp0 f = mk_fun "Tp0" [f]
+
 
 val hasCard_ar = Tp0 hasCard
 
@@ -965,14 +690,6 @@ once_rw [GSYM p32_def] >>
 
 
 
-val Pre_ex = prove_store("Pre_ex",
-e0
-(rpt strip_tac >> qexistsl_tac [‘PRE o n’] >> rw[])
-(form_goal “!X n:X->N. ?pn. PRE o n = pn”));
-
-val Pre_def = Pre_ex |> spec_all |> ex2fsym0 "Pre" ["n"]
-                     |> gen_all |> store_as "Pre_def";
-
 val IN_o = prove_store("IN_o",
 e0
 (rw[IN_def,GSYM Mem_def,GSYM Tp0_def,o_assoc,Pa_distr,True1TRUE,idL] >> once_rw[one_to_one_id] >> rw[idR])
@@ -1011,7 +728,7 @@ e0
 (rw[hasCard_property1] >> rpt strip_tac >> arw[])
 (form_goal “!X.hasCard(X) o Pa(Empty(X),O) = TRUE ”));
 
-
+ 
 
 val hasCard_Ins = prove_store("hasCard_Ins",
 e0
