ETCSZarith.sml
@@ -1,0 +1,1430 @@
+
+val ZR_subset_ex = 
+    pred_subset_ex' |> allE $ rastt "(N * N) * (N * N)"
+                   |> allE $ rastt $ q2str
+‘Eq(N) o Pa(ADD o 
+     Pa(p1(N,N) o p1(N * N,N * N),
+        p2(N,N) o p2(N * N,N * N)),
+     ADD o 
+     Pa(p2(N,N) o p1(N * N,N * N), 
+        p1(N,N) o p2(N * N,N * N)))’
+
+val ZR_subset_def = ex2fsym "ZR" [] (iffRL $ eqT_intro $ spec_all ZR_subset_ex)
+                        |> C mp (trueI []) |> gen_all
+
+val ZRI_def = 
+ex2fsym "ZRI" [] (iffRL $ eqT_intro $ spec_all ZR_subset_def)
+                        |> C mp (trueI []) |> gen_all
+
+val ZRI_Mono = conjE1 ZRI_def
+                      |> store_as "ZRI_Mono";
+
+val Z_ex = 
+    iscoEq_ex |> allE $ rastt "ZR" 
+            |> allE $ rastt "N * N"
+            |> allE $ rastt "p1(N * N, N * N) o ZRI"
+            |> allE $ rastt "p2(N * N, N * N) o ZRI"
+
+val Z_def = ex2fsym "Z" [] (iffRL $ eqT_intro $ spec_all Z_ex)
+                        |> C mp (trueI []) |> gen_all
+
+val toZ_def = ex2fsym "toZ" [] (iffRL $ eqT_intro $ spec_all Z_def)
+                        |> C mp (trueI []) |> gen_all
+
+(*val _ = new_fun "Pow" (ob_sort,[("A",ob_sort)])*)
+
+val ADDj_ex = prove_store("ADDj_ex",
+e0
+(qexists_tac
+ ‘Pa(ADD o Pa(p1(N,N) o p1(N * N,N * N),
+             p1(N,N) o p2(N * N,N * N)) , 
+    ADD o Pa(p2(N,N) o p1(N * N,N * N),
+             p2(N,N) o p2(N * N,N * N)))’ >> rw[])
+(form_goal
+ “?addj. 
+ Pa(ADD o Pa(p1(N,N) o p1(N * N,N * N),
+             p1(N,N) o p2(N * N,N * N)) , 
+    ADD o Pa(p2(N,N) o p1(N * N,N * N),
+             p2(N,N) o p2(N * N,N * N)))= addj”));
+
+
+val ADDj_def = ex2fsym0 "ADDj" [] ADDj_ex;
+
+
+val toZ_Epi = prove_store("toZ_Epi",
+e0
+(assume_tac toZ_def >>
+ drule coEqa_Epi >> first_x_assum accept_tac)
+(form_goal
+ “Epi(toZ)”));
+
+
+val REP_ex = prove_store("REP_ex",
+e0
+(assume_tac toZ_Epi >> drule Epi_has_section >>
+ first_x_assum accept_tac)
+(form_goal 
+ “?rep. toZ o rep = id(Z)”));
+
+val REP_def = REP_ex|> ex2fsym0 "REP" []
+                    |> store_as "REP_def";
+
+val ADDz_ex = prove_store("ADDz_ex",
+e0
+(qexists_tac ‘toZ o ADDj o Pa(REP o p1(Z,Z),REP o p2(Z,Z))’ >>
+ rw[])
+(form_goal
+ “?addz. toZ o ADDj o Pa(REP o p1(Z,Z),REP o p2(Z,Z)) = addz”));
+
+
+
+val ADDz_def = ADDz_ex |> ex2fsym0 "ADDz" []
+                       |> store_as "ADDz_def";
+
+
+
+
+val ADDj_SYM = prove_store("ADDj_SYM",
+e0
+(rw[GSYM Swap_def] >>
+ irule FUN_EXT >> rpt strip_tac >>
+ qby_tac
+ ‘?a0 b0 c0 d0.a = Pa(Pa(a0,b0),Pa(c0,d0))’
+ >-- cheat >>
+ pop_assum strip_assume_tac >> arw[] >>
+ rw[GSYM ADDj_def] >> rw[Pa_distr,o_assoc,p12_of_Pa] >> 
+ qspecl_then [‘c0’,‘a0’] assume_tac ADD_SYM >>
+ qspecl_then [‘d0’,‘b0’] assume_tac ADD_SYM >> 
+ arw[]
+ )
+(form_goal
+ “ADDj o Swap(N * N,N * N) = ADDj”));
+
+
+val ADDz_SYM = prove_store("ADDz_SYM",
+e0
+(rpt strip_tac >>
+ rw[GSYM ADDz_def,o_assoc,Pa_distr,p12_of_Pa] >> 
+ qsuff_tac
+ ‘ADDj o Pa(REP o z1,REP o z2) = 
+  ADDj o Pa(REP o z2,REP o z1)’ 
+ >-- (strip_tac >> arw[]) >>
+ qby_tac
+ ‘ADDj o Pa(REP o z1, REP o z2) = 
+  ADDj o Swap(N * N,N * N) o Pa(REP o z2, REP o z1)’
+ >-- (rw[GSYM Swap_def,Pa_distr,p12_of_Pa,o_assoc]) >>
+ arw[] >> rw[GSYM o_assoc,ADDj_SYM])
+(form_goal
+ “!z1:1->Z z2:1->Z. ADDz o Pa(z1,z2) = ADDz o Pa(z2,z1)”));
+
+
+
+
+val ZR_Refl = prove_store("ZR_Refl",
+e0
+(rw[Refl_Diag] >>
+ rw[GSYM to_P_component] >> 
+ fconv_tac 
+ (basic_once_fconv no_conv (rewr_fconv (eq_sym "ar")))>>
+ rw[GSYM ZRI_def] >> 
+ irule FUN_EXT >> strip_tac >>
+ qsspecl_then [‘a’] assume_tac has_components >>
+ pop_assum strip_assume_tac >>
+ arw[] >>
+ rw[o_assoc,Pa_distr,p12_of_Pa,GSYM Diag_def,idL,
+    GSYM True_def] >>
+ once_rw[one_to_one_id] >> rw[idR] >>
+ rw[Eq_property_TRUE] >> 
+ qsspecl_then [‘a'’,‘b’] accept_tac ADD_SYM
+ )
+(form_goal “Refl(p1(N * N, N * N) o ZRI,p2(N * N, N * N) o ZRI)”));
+
+
+
+
+val ZR_Sym = prove_store("ZR_Sym",
+e0
+(rw[Sym_alt,GSYM to_P_component,p21_Swap] >>
+ irule prop_2_half2 >> 
+ assume_tac ZRI_Mono >>
+ drule Swap_Mono >> arw[] >>
+ rpt strip_tac >>
+ dflip_tac >>  rw[GSYM ZRI_def] >>
+ qby_tac
+ ‘Swap(N * N,N * N) o (Swap(N * N, N * N) o ZRI) o xb = 
+  Swap(N * N, N * N) o x’
+ >-- arw[] >>
+ pop_assum mp_tac >> rw[GSYM o_assoc,Swap_Swap_id,idL]>>
+ strip_tac >>
+ qby_tac 
+ ‘?xb. Swap(N * N,N * N) o x = ZRI o xb’ 
+ >-- (qexists_tac ‘xb’ >> arw[]) >>
+ pop_assum mp_tac >>
+ rw[GSYM ZRI_def,True1TRUE] >>
+ rw[Eq_property_TRUE,o_assoc,Pa_distr,p12_of_Pa] >>
+ qsspecl_then [‘x’] strip_assume_tac has_components >>
+ qsspecl_then [‘a’] strip_assume_tac has_components >>
+ qsspecl_then [‘b’] strip_assume_tac has_components >>
+ arw[p12_of_Pa] >>
+ rw[GSYM Swap_def,o_assoc,Pa_distr,p12_of_Pa] >>
+ strip_tac >>
+ qsspecl_then [‘a''’,‘b'’] assume_tac ADD_SYM >> fs[] >>
+ qsspecl_then [‘b''’,‘a'’] assume_tac ADD_SYM >> fs[] )
+(form_goal “Sym(p1(N * N, N * N) o ZRI,p2(N * N, N * N) o ZRI)”));
+
+
+
+
+
+
+
+(*
+local 
+val l =
+fVar_Inst 
+[("P",([("m",mem_sort N)],
+ “!n0 p. Add(m,Add(n0,p)) = Add(Add(m,n0),p)”))] 
+N_ind_P
+in
+val Add_assoc = prove_store("Add_assoc",
+e0
+(irule l >> rw[Add_O,Suc_def,Add_Suc,Add_Suc1,Add_O2] >>
+ rpt strip_tac >>arw[])
+(form_goal
+ “!m n0 p. Add(m,Add(n0,p)) = Add(Add(m,n0),p)”));
+end
+
+*)
+
+val ADD_assoc = prove_store("ADD_assoc",
+e0
+(assume_tac equality_ind >>
+ pop_assum (qspecl_then [‘N * N’,‘N’,‘ADD o Pa(p2(N * N,N),ADD o p1(N * N,N))’,‘N * N’,‘ADD o Pa(ADD o Pa(p2(N * N,N),p1(N,N) o p1(N * N,N)), p2(N,N) o p1(N * N,N))’] assume_tac) >> 
+ qsuff_tac
+ ‘!n0:1->N p m.ADD o Pa(m, ADD o Pa(n0,p)) = 
+           ADD o Pa(ADD o Pa(m,n0),p)’
+ >-- (strip_tac >>  arw[]) >>
+ strip_tac >> strip_tac >>
+ first_x_assum
+ (qsspecl_then [‘Pa(n0,p)’,‘Pa(n0,p)’] assume_tac) >>
+ fs[Pa_distr,o_assoc,p12_of_Pa] >>
+ pop_assum (K all_tac) >>
+ rw[ADD_O_n,ADD_el,ADD_SUC] >> rpt strip_tac >>
+ arw[])
+(form_goal
+ “!m:1->N n0 p. ADD o Pa(m, ADD o Pa(n0,p)) = 
+           ADD o Pa(ADD o Pa(m,n0),p)”));
+
+val ZR_Trans =prove_store("ZR_Trans",
+e0
+(assume_tac ZRI_Mono >>
+ irule $ iffRL Trans_alt' >> rw[GSYM to_P_component]>>
+ arw[] >> dflip_tac >> rpt strip_tac >>
+ qby_tac
+ ‘?r01. Pa(h0, h1) = ZRI o r01’
+ >-- (qexists_tac ‘r01’ >> arw[]) >>
+ qby_tac
+ ‘?r12. Pa(h1, h2) = ZRI o r12’
+ >-- (qexists_tac ‘r12’ >> arw[]) >>
+ pop_assum mp_tac >> pop_assum mp_tac >>
+ rw[GSYM ZRI_def,True1TRUE,Pa_distr,
+    Eq_property_TRUE,o_assoc,p12_of_Pa] >> 
+ qsspecl_then [‘h0’] assume_tac has_components >> 
+ pop_assum strip_assume_tac >>
+ qsspecl_then [‘h1’] assume_tac has_components >> 
+ pop_assum strip_assume_tac >> 
+ qsspecl_then [‘h2’] assume_tac has_components >> 
+ pop_assum strip_assume_tac >>
+ arw[p12_of_Pa] >> rpt strip_tac >>
+ qby_tac
+ ‘ADD o Pa(ADD o Pa(a, b''),b') = 
+  ADD o Pa(a,ADD o Pa(b',b''))’
+ >-- (qspecl_then [‘b'’,‘b''’] assume_tac ADD_SYM >>
+      arw[] >> rw[ADD_assoc]) >>
+ fs[ADD_assoc] >> rfs[] >>
+ fs[GSYM ADD_assoc] >> rfs[] >>
+ qspecl_then [‘b'’,‘a''’] assume_tac ADD_SYM >> fs[] >>
+ fs[ADD_assoc] >>
+ assume_tac ADD_SUB >>
+ first_assum (qspecl_then [‘ADD o Pa(a, b'')’,‘b'’]
+ assume_tac) >>
+ first_x_assum (qspecl_then [‘ADD o Pa(b, a'')’,‘b'’]
+ assume_tac) >>
+ pop_assum (assume_tac o GSYM) >>once_arw[] >>
+ pop_assum (K all_tac) >>
+ pop_assum (assume_tac o GSYM) >> once_arw[] >>
+ pop_assum (K all_tac) >>
+ arw[])
+(form_goal
+ “Trans(p1(N * N, N * N) o ZRI,p2(N * N, N * N) o ZRI)”));
+
+val Thm6_ZR = prove_store("Thm6_ZR",
+e0
+(assume_tac Thm6_isEq >> 
+ qby_tac ‘ZRI =  Pa(p1(N * N, N * N) o ZRI, p2(N * N, N * N) o ZRI)’
+ >-- rw[GSYM to_P_component] >> once_arw[] >>
+ first_x_assum irule >> rw[GSYM to_P_component] >> 
+ rw[ZRI_Mono,ZR_Trans,ZR_Sym,ZR_Refl,toZ_def])
+(form_goal
+ “isEq(toZ o p1(N * N, N * N),toZ o p2(N * N,N * N),ZRI)”));
+
+
+val Addz_ex = prove_store("Addz_ex",
+e0
+(rpt strip_tac >> qexists_tac ‘ADDz o Pa(z1,z2)’ >> rw[])
+(form_goal
+ “!X z1:X->Z z2. ?z12. ADDz o Pa(z1,z2) = z12”));
+
+val Addz_def = Addz_ex |> spec_all |> ex2fsym0 "Addz" ["z1","z2"]
+                       |> gen_all |> store_as "Addz_def";
+
+val asz_ex = prove_store("asz_ex",
+e0
+(rpt strip_tac >> qexists_tac ‘toZ o pair’ >> rw[])
+(form_goal “!X pair:X-> N * N. ?z. toZ o pair= z”));
+
+val asz_def = asz_ex |> spec_all |> ex2fsym0 "asz" ["pair"]
+                     |> gen_all |> store_as "asz_def";
+
+
+val Addj_ex = prove_store("Addj_ex",
+e0
+(rpt strip_tac >> qexists_tac ‘ADDj o Pa(ab,cd)’ >> rw[])
+(form_goal “!X ab:X->N * N cd. ?acbd.ADDj o Pa(ab,cd) = acbd”));
+
+val Addj_def = Addj_ex |> spec_all |> ex2fsym0 "Addj" ["ab","cd"]
+                       |> gen_all |> store_as "Addj_def";
+
+val _ = new_pred "ZR" [("ab",ar_sort (mk_ob "X") (Po N N)),
+                       ("cd",ar_sort (mk_ob "X") (Po N N))]
+
+val ZR_def0 = store_ax("ZR_def0",
+“!X ab:X->N * N cd. ZR(ab,cd) <=> ?x0:X-> ZR.Pa(ab,cd) = ZRI o x0”);
+
+
+val Add_ex = prove_store("Add_ex",
+e0
+(rpt strip_tac >> qexists_tac ‘ADD o Pa(a,b)’ >> rw[])
+(form_goal
+ “!a:X->N b. ?ab. ADD o Pa(a,b) = ab”));
+
+val Add_def = Add_ex |> spec_all |> ex2fsym0 "Add" ["a","b"]
+                     |> gen_all
+                     |> store_as "Add_def";
+
+val Fst_ex = prove_store("Fst_ex",
+e0
+(rpt strip_tac >> qexists_tac ‘p1(A,B) o ab’ >> rw[])
+(form_goal “!X A B ab:X->A * B. ?fst.p1(A,B) o ab = fst”));
+
+
+val Snd_ex = prove_store("Snd_ex",
+e0
+(rpt strip_tac >> qexists_tac ‘p2(A,B) o ab’ >> rw[])
+(form_goal “!X A B ab:X->A * B. ?snd.p2(A,B) o ab = snd”));
+
+val Fst_def = Fst_ex |> spec_all |> ex2fsym0 "Fst" ["ab"]
+                     |> gen_all
+                     |> store_as "Fst_def";
+
+
+
+val Snd_def = Snd_ex |> spec_all |> ex2fsym0 "Snd" ["ab"]
+                     |> gen_all
+                     |> store_as "Snd_def";
+
+val Fst_Snd_Pa = p12_of_Pa |> rewr_rule[Fst_def,Snd_def]
+                           |> store_as "Fst_Snd_Pa";
+
+val Fst_Pa = p1_of_Pa |> rewr_rule[Fst_def] |> store_as "Fst_Pa";
+
+val Snd_Pa = p2_of_Pa |> rewr_rule[Snd_def] |> store_as "Snd_Pa";
+
+val ZR_def = prove_store("ZR_def",
+e0
+(rpt strip_tac >> 
+ rw[ZR_def0,GSYM ZRI_def,GSYM Eq_property,p12_of_Pa,Pa_distr,o_assoc] >>
+ qsspecl_then [‘ab’] strip_assume_tac has_components >>
+ qsspecl_then [‘cd’] strip_assume_tac has_components >> arw[p12_of_Pa,Fst_Snd_Pa] >> dimp_tac >> strip_tac >> fs[GSYM Add_def])
+(form_goal
+ “!X ab:X->N * N cd. ZR(ab,cd) <=> 
+  Add(Fst(ab),Snd(cd)) = Add(Snd(ab),Fst(cd))”));
+
+
+val rep_ex = prove_store("rep_ex",
+e0
+(rpt strip_tac >> qexists_tac ‘REP o z’ >> rw[] )
+(form_goal “!X z:X->Z.?r. REP o z = r”));
+
+val rep_def= rep_ex |> spec_all |> ex2fsym0 "rep" ["z"] 
+                    |> gen_all |> store_as "rep_def";
+
+val rep_asz = prove_store("rep_asz",
+e0
+(rpt strip_tac >> rw[GSYM rep_def,GSYM asz_def,REP_def,GSYM o_assoc,idL])
+(form_goal “!X z:X->Z. asz(rep(z)) = z”)); 
+
+(*asz_def rep_def toZ_def REP_def*)
+
+val lflip_tac =
+fconv_tac 
+ (land_fconv no_conv 
+ $ basic_once_fconv no_conv (rewr_fconv (eq_sym "ar")))
+
+val rflip_tac =
+fconv_tac 
+ (rand_fconv no_conv 
+ $ basic_once_fconv no_conv (rewr_fconv (eq_sym "ar")))
+
+
+
+val samez_cond = prove_store("samez_cond",
+e0
+(rw[ZR_def,GSYM asz_def] >> 
+ assume_tac Thm6_ZR >> drule via_Eq_iff >> 
+ rpt strip_tac >>
+ (*qsspecl_then [‘ab’] strip_assume_tac has_components >>
+ qsspecl_then [‘cd’] strip_assume_tac has_components >> fs[] >> *)
+ first_x_assum (qsspecl_then [‘Pa(ab,cd)’] assume_tac) >> fs[o_assoc,p12_of_Pa] >>
+ pop_assum (assume_tac o GSYM) >> arw[] >> lflip_tac >> 
+ rw[GSYM ZR_def] >> rw[ZR_def0])
+(form_goal “!X ab:X-> N * N cd. asz(ab) = asz(cd) <=> ZR(ab,cd)”));
+
+val ZR_samez = GSYM samez_cond;
+
+val rep_asz_ZR = prove_store("rep_asz_ZR",
+e0
+(rw[GSYM samez_cond,rep_asz])
+(form_goal “!X ab:X->N * N.ZR(ab,rep(asz(ab)))”));
+
+val rep_ZR_eq = prove_store("rep_ZR_eq",
+e0
+(rw[ZR_samez,rep_asz])
+(form_goal
+ “!X z1:X->Z z2. ZR(rep(z1),rep(z2)) <=> z1 = z2”));
+
+val z_eq_cond = prove_store("z_eq_cond",
+e0
+(rpt strip_tac >> dimp_tac >> strip_tac (* 2 *)
+ >-- (qexistsl_tac [‘rep(z1)’,‘rep(z2)’] >> arw[rep_asz,rep_ZR_eq]) >>
+ fs[ZR_samez])
+(form_goal “!X z1:X->Z z2. z1 = z2 <=> ?ab cd. asz(ab) = z1 & asz(cd) = z2 & ZR(ab,cd) ”));
+
+val Add_sym = ADD_SYM |> rewr_rule[Add_def] |> store_as "Add_sym";
+
+val ZR_refl = prove_store("ZR_refl",
+e0
+(rw[ZR_def] >> rpt strip_tac >>
+ qsspecl_then [‘Fst(ab)’,‘Snd(ab)’] assume_tac Add_sym >> arw[])
+(form_goal “!ab:1->N * N.ZR(ab,ab)”));
+
+
+val ZR_sym = prove_store("ZR_sym",
+e0
+(rw[ZR_def] >> rpt strip_tac >> lflip_tac >>
+ qsspecl_then [‘Fst(ab)’,‘Snd(cd)’] assume_tac Add_sym >> arw[] >> 
+ qsspecl_then [‘Fst(cd)’,‘Snd(ab)’] assume_tac Add_sym >> arw[])
+(form_goal “!ab:1->N * N cd.ZR(ab,cd) <=> ZR(cd,ab)”));
+
+
+val ZR_trans = prove_store("ZR_sym",
+e0
+(assume_tac ZR_Trans >> 
+ assume_tac ZRI_Mono >>
+ pop_assum mp_tac >> once_rw[to_P_component] >> strip_tac >> 
+ drule Trans_alt' >> fs[GSYM to_P_component] >> pop_assum (K all_tac) >>
+ rw[ZR_def0] >> rpt strip_tac >> dflip_tac >> first_x_assum irule >>
+ qexistsl_tac [‘cd’,‘x0’,‘x0'’] >> arw[])
+(form_goal “!ab:1->N * N  cd ef.ZR(ab,cd) & ZR(cd,ef) ==> ZR(ab,ef)”));
+
+val ZR_cond = prove_store("ZR_cond",
+e0
+(rpt strip_tac >> dimp_tac >> strip_tac 
+ >-- (qexistsl_tac [‘ab’,‘cd’] >> arw[ZR_refl]) >>
+ qby_tac ‘ZR(ab,cd1)’ 
+ >-- (irule ZR_trans >> qexists_tac ‘ab1’ >> arw[]) >>
+ qby_tac ‘ZR(cd1,cd)’
+ >-- (irule $ iffLR ZR_sym >> arw[]) >>
+ irule ZR_trans >>
+ qexists_tac ‘cd1’ >> arw[])
+(form_goal “!ab:1->N * N cd.ZR(ab,cd) <=> ?ab1 cd1. ZR(ab,ab1) & ZR(cd,cd1) & ZR(ab1,cd1)”));
+
+
+val rep_rel_all = prove_store("rep_rel_all",
+e0
+(rpt strip_tac >> dimp_tac >> strip_tac 
+ >-- (pop_assum (assume_tac o GSYM) >> arw[] >>
+      irule $ iffLR ZR_sym >> rw[rep_asz_ZR]) >>
+ fs[ZR_samez,rep_asz])
+(form_goal
+ “!z:1->Z rz.asz(rz) = z <=> ZR(rep(z),rz)”));
+
+val Pa_Fst_Snd = to_P_component |> rewr_rule[Fst_def,Snd_def] |> GSYM
+                                |> store_as "Pa_Fst_Snd";
+
+val z_has_rep = prove_store("z_has_rep",
+e0
+(strip_tac >> rw[GSYM asz_def] >> rpt strip_tac >>
+ qexistsl_tac [‘Fst(rep(z))’,‘Snd(rep(z))’] >>
+ rw[Pa_Fst_Snd] >> rw[asz_def,rep_asz])
+(form_goal
+ “!X z:X->Z. ?a b. z = asz(Pa(a,b))”));
+
+
+val Add_assoc = ADD_assoc |> rewr_rule[Add_def] |> store_as "Add_assoc";
+
+val Addj_property =  prove_store("Addj_property",
+e0
+(rw[GSYM Addj_def,GSYM ADDj_def,p12_of_Pa,Pa_distr,o_assoc,GSYM Add_def])
+(form_goal
+ “!a:1->N b c d. Addj(Pa(a,b),Pa(c,d)) = Pa(Add(a,c),Add(b,d))”));
+
+
+val J1_i = prove_store("J1_i",
+e0
+(rw[ZR_def,Addj_property] >> rpt strip_tac >> 
+ rw[Fst_Snd_Pa] >>
+ qsspecl_then [‘Add(Add(a, c), e)’,‘Add(b, Add(d, f))’] assume_tac Add_sym >>
+ arw[] >> rw[GSYM Add_assoc])
+(form_goal “!a b c d e f:1->N. 
+ ZR(Addj(Addj(Pa(a,b),Pa(c,d)),Pa(e,f)),
+    Addj(Pa(a,b),Addj(Pa(c,d),Pa(e,f))))”));
+
+
+val ZR_def' = prove_store("ZR_def'",
+e0
+(rw[ZR_def] >> rpt strip_tac >> 
+ qsspecl_then [‘Snd(ab)’,‘Fst(cd)’] assume_tac Add_sym >>
+ arw[])
+(form_goal
+ “!ab:1 ->N * N cd.
+        ZR(ab, cd) <=> Add(Fst(ab), Snd(cd)) = Add(Fst(cd), Snd(ab))”));
+
+val Add_sym' = GSYM Add_sym
+
+val J2_i = prove_store("J2_i",
+e0
+(rw[Addj_property,ZR_def',Fst_Snd_Pa] >>
+ rpt strip_tac >>
+ rw[GSYM Add_assoc] >>
+ qspecl_then [‘d'’,‘b'’] assume_tac Add_sym' >> arw[] >>
+ qspecl_then [‘c’,‘d'’,‘b'’] assume_tac Add_assoc >>
+ arw[] >>
+ rw[GSYM Add_assoc] >>
+ qspecl_then [‘Add(c',Add(d,b'))’,‘a’] assume_tac Add_sym' >> 
+ arw[] >>
+ rw[GSYM Add_assoc] >>
+ qspecl_then [‘a’,‘b'’] assume_tac Add_sym' >>
+ arw[] >>
+ qsspecl_then [‘Add(c', Add(b, d))’,‘a'’]
+ assume_tac Add_sym' >> arw[] >>
+ rw[GSYM Add_assoc] >> 
+ qsuff_tac
+ ‘Add(d, Add(a', b)) = Add(b, Add(d, a'))’
+ >-- (strip_tac >> arw[]) >>
+ qspecl_then [‘Add(a',b)’,‘d’] assume_tac Add_sym' >>
+ arw[] >> 
+ qspecl_then [‘a'’,‘d’] assume_tac Add_sym' >> arw[] >>
+ rw[Add_assoc] >>
+ qspecl_then [‘a'’,‘b’] assume_tac Add_sym' >> arw[])
+(form_goal
+ “!a:1->N b a' b' c d c' d'. ZR(Pa(a,b),Pa(a',b')) & ZR(Pa(c,d),Pa(c',d')) ==>
+ ZR(Addj(Pa(a,b),Pa(c,d)),Addj(Pa(a',b'),Pa(c',d')))”));
+
+
+val J2_i_z = prove_store("J2_i_z",
+e0
+(rpt strip_tac >> assume_tac J2_i >>
+ rw[GSYM Addz_def,GSYM ADDz_def,o_assoc,Pa_distr] >> rw[asz_def,p12_of_Pa] >>
+ rw[samez_cond] >> arw[] >>
+ rw[rep_def,Addj_def]  >> 
+ qsspecl_then [‘rep(asz(Pa(a,b)))’] strip_assume_tac has_components >>
+ qsspecl_then [‘rep(asz(Pa(c,d)))’] strip_assume_tac has_components >>
+ arw[] >> first_x_assum irule >> pop_assum_list (map_every (assume_tac o GSYM)) >>
+ arw[] >> rw[GSYM rep_rel_all] >> arw[])
+(form_goal
+ “!z1:1->Z z2 a b c d. z1 = asz(Pa(a,b)) & z2 = asz(Pa(c,d)) ==>
+ Addz(z1,z2) = asz(Addj(Pa(a,b),Pa(c,d)))”));
+
+
+val Addz_eqn' = prove_store("Addz_eqn'",
+e0
+(rpt strip_tac >>
+ assume_tac J2_i_z >>
+ first_x_assum irule >> rw[])
+(form_goal
+ “!a:1->N b c d.
+  Addz(asz(Pa(a,b)),asz(Pa(c,d))) = 
+  asz(Addj(Pa(a,b),Pa(c,d)))”));
+
+val ADDz_assoc = prove_store("ADDz_assoc",
+e0
+(rpt strip_tac >> 
+ qsspecl_then [‘z1’] strip_assume_tac z_has_rep >>
+ qsspecl_then [‘z2’] strip_assume_tac z_has_rep >>
+ qsspecl_then [‘z3’] strip_assume_tac z_has_rep >>
+ arw[] >> 
+ rw[Addz_eqn'] >> rw[Addj_property] >>
+ rw[Addz_eqn'] >> rw[GSYM Addj_property] >>
+ assume_tac J1_i >> fs[ZR_samez])
+(form_goal
+ “!z1:1->Z z2 z3. Addz(Addz(z1,z2),z3) = Addz(z1,Addz(z2,z3))”));
+
+
+
+
+val zj_ex = prove_store("zj_ex",
+e0
+(qexists_tac ‘Pa(O,O)’ >> rw[])
+(form_goal
+ “?zj.Pa(O,O) = zj”));
+
+val zj_def = zj_ex |> ex2fsym0 "0j" []
+                   |> store_as "zj_def";
+
+
+
+val NEGj_ex = prove_store("NEGj_ex",
+e0
+(rpt strip_tac >> qexists_tac ‘Swap(N,N)’ >> rw[])
+(form_goal “?NEGj.Swap(N,N) =NEGj ”));
+
+val NEGj_def = NEGj_ex |> spec_all |> ex2fsym0 "NEGj" []
+                       |> gen_all |> store_as "NEGj_def";
+
+
+
+val NEGj_property = prove_store("NEGj_property",
+e0
+(rpt strip_tac >> rw[GSYM NEGj_def,Swap_Pa])
+(form_goal “!X a:X->N b. NEGj o Pa(a,b) = Pa(b,a)”));
+
+
+val Negj_ex = prove_store("Negj_ex",
+e0
+(rpt strip_tac >> qexists_tac ‘NEGj o ab’ >> rw[])
+(form_goal “!X ab:X->N * N. ?nab. NEGj o ab = nab”));
+
+val Negj_def = Negj_ex |> spec_all |> ex2fsym0 "Negj" ["ab"] 
+                       |> gen_all |> store_as "Negj_def";
+
+val Negj_property = NEGj_property |> rewr_rule[Negj_def]
+
+
+val Add_El = ADD_el |> rewr_rule [Add_def] |> store_as "Add_El";
+
+val Add_O_n = ADD_O_n |> rewr_rule[Add_def] |> store_as "Add_O_n";
+
+
+val J1_ii = prove_store("J1_ii",
+e0
+(rw[GSYM zj_def,Addj_property,ZR_def,Fst_Snd_Pa,Add_O_n,Add_El] >> rpt strip_tac >>
+ qsspecl_then [‘a’,‘b’] accept_tac Add_sym)
+(form_goal
+ “!a b.ZR(Addj(Pa(a,b),0j),Pa(a,b))”));
+
+
+val zz_ex = prove_store("zz_ex",
+e0
+(qexists_tac ‘asz(0j)’ >> rw[])
+(form_goal
+ “?z. asz(0j) = z”));
+
+val zz_def = zz_ex |> ex2fsym0 "0z" []
+                   |> store_as "zz_def";
+
+
+val Addz_zz = prove_store("Addz_zz",
+e0
+(strip_tac >> once_rw[z_eq_cond] >>
+ qsspecl_then [‘z’] strip_assume_tac z_has_rep >> 
+ arw[] >>
+ assume_tac J1_ii >>
+ fs[ZR_samez] >> 
+ rw[GSYM zz_def] >> rw[GSYM zj_def,Addz_eqn'] >>
+ rw[zj_def] >> arw[] >>
+ qexistsl_tac [‘Pa(a,b)’,‘Pa(a,b)’] >> rw[])
+(form_goal
+ “!z. Addz(z,0z) = z”));
+
+val Z2_ii = Addz_zz |> store_as "Z2_ii";
+
+val Negz_ex =  prove_store("Negz_ex",
+e0
+(rpt strip_tac >> qexists_tac ‘asz(Negj(rep(z)))’ >> rw[])
+(form_goal “!X z:X->Z.?nz. asz(Negj(rep(z))) = nz”));
+
+val Negz_def = Negz_ex |> spec_all |> ex2fsym0 "Negz" ["z"]
+                       |> gen_all |> store_as "Negz_def";
+
+
+val J2_ii = prove_store("J2_ii",
+e0
+(rw[ZR_def,Negj_property,Fst_Snd_Pa] >>rpt strip_tac >> arw[])
+(form_goal
+ “!X a:X->N b a' b'. ZR(Pa(a,b),Pa(a',b')) ==> 
+  ZR(Negj(Pa(a,b)),Negj(Pa(a',b')))”));
+
+
+val J2_ii_z = prove_store("J2_ii_z",
+e0
+(rpt strip_tac >> assume_tac J2_ii >>
+ rw[GSYM Negz_def] >> rw[samez_cond] >> 
+ qsspecl_then [‘rep(z)’] strip_assume_tac has_components >> arw[] >>
+ first_x_assum irule >> pop_assum (assume_tac o GSYM) >> arw[] >>
+ rw[GSYM rep_rel_all])
+(form_goal
+ “!a:1->N b z. z = asz(Pa(a,b)) ==>
+  Negz(z) = asz(Negj(Pa(a,b)))”));
+
+
+val Negz_eqn = prove_store("Negz_eqn",
+e0
+(rpt strip_tac >> irule J2_ii_z >> arw[])
+(form_goal
+ “!a:1->N b. Negz(asz(Pa(a,b))) = asz(Negj(Pa(a,b)))”));
+
+
+val J1_iii = prove_store("J1_iii",
+e0
+(rw[Addj_property,GSYM zj_def,Negj_property,ZR_def,
+    Fst_Snd_Pa,Add_El,Add_O_n] >>
+ rpt strip_tac >>
+ qspecl_then [‘a’,‘b’] assume_tac Add_sym >>
+ first_x_assum accept_tac)
+(form_goal
+ “!a b. ZR(Addj(Pa(a,b),Negj(Pa(a,b))),0j)”));
+
+
+
+val Z2_iii = prove_store("Z2_iii",
+e0
+(rpt strip_tac >>
+ qsspecl_then [‘z’] strip_assume_tac z_has_rep >> 
+ arw[] >> rw[Negz_eqn,Addz_eqn',Negj_property,Addj_property] >> rw[GSYM zz_def]  >>
+ rw[GSYM ZR_samez,ZR_def,Fst_Snd_Pa,GSYM zj_def,Add_El,Add_O_n] >>
+ qspecl_then [‘a’,‘b’] accept_tac Add_sym)
+(form_goal
+ “!z. Addz(z,Negz(z)) = 0z”));
+
+val _ = new_pred "Le" [("m",ar_sort (mk_ob "X") N),
+                       ("n",ar_sort (mk_ob "X") N)]
+
+val Le_def0 = store_ax("Le_def0",
+ “!X a:X->N b:X->N. Le(a,b) <=> Char(LE) o Pa(a,b) = True(X)”);
+
+
+val Le_def1 = Le_def0 |> allE (rastt "1")
+                      |> rewr_rule[True1TRUE]
+
+val _ = new_pred "Lt" [("m",ar_sort (mk_ob "X") N),
+                       ("n",ar_sort (mk_ob "X") N)]
+
+val Lt_def0 = store_ax("Lt_def0",
+ “!X a:X->N b:X->N. Lt(a,b) <=> Char(LT) o Pa(a,b) = True(X)”);
+
+
+val Lt_def1 = Lt_def0 |> allE (rastt "1")
+                     |> rewr_rule[True1TRUE]
+
+
+val Le_def = LE_SUB |> rewr_rule[GSYM Le_def1,Sub_def]
+
+val Lt_def = prove_store("Lt_def",
+e0
+(rw[Lt_def1,CLT_iff_LE_NE,Le_def1,LE_Char_LEo])
+(form_goal 
+ “!a:1->N b. Lt(a,b) <=> Le(a,b) & ~(a = b)”));
+
+val Sub_of_O = SUB_0 |> rewr_rule[Sub_def]
+                     |> store_as "Sub_of_O";
+
+val Sub_O = SUB_0_cj2 |> rewr_rule[Sub_def]
+                      |> store_as "Sub_O";
+
+val Add_O = ADD_el |> spec_all |> conjE1
+                   |> gen_all 
+                   |> rewr_rule[Add_def]
+                   |> store_as "Add_O";
+
+
+val Add_Suc = ADD_el |> spec_all |> conjE2
+                   |> gen_all 
+                   |> rewr_rule[Add_def,Suc_def]
+                   |> store_as "Add_O";
+
+val Add_O2 = ADD_O_n |> rewr_rule[Add_def]
+                      |> store_as "Add_O2";
+
+val Add_Suc1 = ADD_SUC |> rewr_rule[Add_def,Suc_def]
+                       |> store_as "Add_Suc1";
+
+val Sub_mono_eq = SUB_MONO_EQ
+                      |> rewr_rule[Sub_def,Suc_def]
+                      |> store_as "Sub_mono_eq";
+
+val Sub_Add = prove_store("Sub_Add",
+e0
+(qby_tac
+ ‘?P0. !c b a:1->N. P0 o Pa3(c,b,a) = TRUE <=> 
+  Sub(a,Add(b,c)) = Sub(Sub(a,b),c)’ >-- 
+ (qexists_tac 
+ ‘Eq(N) o Pa(SUB o Pa(p33(N,N,N),ADD o Pa(p32(N,N,N),p31(N,N,N))),SUB o Pa(SUB o Pa(p33(N,N,N),p32(N,N,N)),p31(N,N,N)))’ >>
+  once_rw[GSYM Pa3_def] >> 
+  once_rw[GSYM p31_def] >> once_rw[GSYM p32_def] >>
+  once_rw[o_assoc] >> once_rw[Pa_distr] >>
+  once_rw[Eq_property_TRUE] >> 
+  once_rw[GSYM p33_def] >>
+  rw[o_assoc,p12_of_Pa,Pa_distr] >>
+  rw[Sub_def,Add_def]) >>
+ pop_assum strip_assume_tac >>
+ qsuff_tac 
+ ‘!a b c. P0 o Pa3(c,b,a) = TRUE’
+ >-- (rpt strip_tac >> fs[]) >>
+ rw[triple_IND',GSYM Pa3_def] >>
+ fs[GSYM Pa3_def] >> rw[Suc_def] >>
+ rw[Sub_of_O] >> strip_tac >> strip_tac >> 
+ strip_tac (* 2 *)
+ >-- rw[Sub_O,Add_O2] >>
+ rpt strip_tac (* 2 *)
+ >-- rw[Sub_O,Add_O] >>
+ rw[Add_Suc1] >> rw[Sub_mono_eq] >> arw[])
+(form_goal
+ “!a:1->N b c. Sub(a,Add(b,c)) = Sub(Sub(a,b),c)”));
+
+val Le_O_iff = prove_store("Le_O_iff",
+e0
+(strip_tac >> dimp_tac >> strip_tac 
+ >-- (fs[Le_def1] >> drule LE_O_O >> arw[]) >>
+ arw[] >> rw[Le_def] >> rw[Sub_O])
+(form_goal
+ “!a. Le(a,O) <=> a = O”));
+
+val Le_cases = LE_cases 
+                   |> rewr_rule[GSYM Le_def1,
+                                GSYM Lt_def1]
+                   |> store_as "Le_cases";
+
+val Lt_Suc_Le = LESS_SUC_LEQ 
+                    |> rewr_rule[GSYM Le_def1,
+                                GSYM Lt_def1,
+                                Suc_def]
+                   |> store_as "Lt_Suc_Le";
+
+val Le_Suc = prove_store("Le_Suc",
+e0
+(rpt strip_tac >> drule Le_cases >>
+ pop_assum strip_assume_tac >--
+ (drule $ iffLR Lt_Suc_Le >> arw[]) >> arw[])
+(form_goal 
+ “!a:1->N b. Le(a,Suc(b)) ==> (Le(a,b) | a = Suc(b))”));
+
+
+val Le_Add_ex = prove_store("Le_Add",
+e0
+(qby_tac
+ ‘?P. !n m. P o Pa(n,m) = TRUE <=> 
+  (Le(n,m) ==> ?p. Add(p,n) = m)’
+ >-- cheat >>
+ pop_assum strip_assume_tac >>
+ qsuff_tac
+ ‘!m. ALL(P) o m = TRUE’ 
+ >-- arw[ALL_property] >>
+ rw[IP_el] >> arw[ALL_property,Suc_def,Le_O_iff] >>
+ rpt strip_tac (* 2 *)
+ >-- (arw[] >> qexists_tac ‘O’ >> rw[Add_O]) >>
+ drule Le_Suc >> pop_assum strip_assume_tac (* 2 *)
+ >-- (first_x_assum drule >>
+     pop_assum strip_assume_tac >>
+     qexists_tac ‘Suc(p)’ >> arw[Add_Suc1]) >>
+ arw[] >> qexists_tac ‘O’ >> rw[Add_O2])
+(form_goal
+ “!m:1->N n. Le(n,m) ==> ?p. Add(p,n) = m”));
+
+
+val lej_ex = prove_store("lej_ex",
+e0
+(qexists_tac
+ ‘Char(LE) o Pa(
+  ADD o Pa(p1(N,N) o p1(N * N,N * N),
+           p2(N,N) o p2(N * N,N * N)),
+  ADD o Pa(p2(N,N) o p1(N * N,N * N),
+           p1(N,N) o p2(N * N,N * N))
+)’ >-- rpt strip_tac >>
+ qsspecl_then [‘ab’] assume_tac has_components >>
+ qsspecl_then [‘cd’] assume_tac has_components >>
+ fs[] >> 
+ rw[Pa_distr,p12_of_Pa,o_assoc] >>
+ rw[Le_def1])
+(form_goal
+ “?lej. !ab:1->N * N cd. 
+  lej o Pa(ab,cd) = TRUE <=> 
+  Le(ADD o Pa(p1(N,N) o ab,p2(N,N) o cd),
+     ADD o Pa(p2(N,N) o ab,p1(N,N) o cd))”));
+
+val lej_def = ex2fsym0 "lej" [] lej_ex
+                       |> store_as "lej_def";
+
+val Le_trans = prove_store("Le_trans",
+e0
+(rpt strip_tac >> rw[Le_def] >>
+ drule Le_Add_ex >> pop_assum (strip_assume_tac o GSYM)>>
+ arw[] >> 
+ qsspecl_then [‘p’,‘b’] assume_tac Add_sym >>
+ once_arw[] >> rw[Sub_Add] >> fs[Le_def] >>
+ rw[Sub_of_O])
+(form_goal
+ “!a:1->N b c. Le(a,b) & Le(b,c) ==> Le(a,c)”));
+
+val Lt_mono_eq = 
+LESS_MONO_EQ 
+    |> rewr_rule[GSYM Lt_def1,Suc_def]
+    |> store_as "Lt_mono_eq";
+
+val LESS_MONO_ADD = prove_store("LESS_MONO_ADD",
+e0
+(strip_tac >> strip_tac >>
+qby_tac
+ ‘?P. !p.  
+ P o p = TRUE <=> 
+ (Lt(m,n) <=> Lt(Add(m,p),Add(n,p))) ’
+ >-- (
+ qexists_tac ‘Iff(Char(LT) o Pa(m,n) o To1(N),
+              Char(LT) o 
+              Pa(ADD o Pa(m o To1(N),id(N)),
+                 ADD o Pa(n o To1(N),id(N))))’
+ >-- rw[GSYM Iff_def,Pa_distr,p12_of_Pa,o_assoc,
+        IFF_def] >>
+     once_rw[one_to_one_id] >> rw[idR,idL] >>
+     rw[GSYM Lt_def1] >> rw[Add_def])>>
+ pop_assum strip_assume_tac >> 
+ qsuff_tac
+ ‘!p. P o p = TRUE’
+ >-- fs[ALL_property] >>
+ rw[IP_el] >> strip_tac >-- 
+ (*  why arw makes no change? after rw[IP_el], if use 
+ arw, no change, and if arw with Suc_def, no change, it use rw, mmakes change*) 
+ arw[Add_O] >> 
+ rw[Suc_def] >> rpt strip_tac >> rfs[]
+ (*the thing that should be done by arw is done by 
+  rfs*)
+ >>fs[Add_Suc,Lt_mono_eq])
+(form_goal
+ “!m:1->N n p. Lt(m,n) <=> Lt(Add(m,p),Add(n,p))”));
+
+val Suc_eq_eq = 
+INV_SUC_EQ |> rewr_rule[Suc_def]
+           |> store_as "Suc_eq_eq";
+
+val EQ_MONO_ADD_EQ = prove_store("EQ_MONO_ADD_EQ",
+e0
+(strip_tac >> strip_tac >>
+qby_tac
+ ‘?P. !p.  
+ P o p = TRUE <=> 
+ Add(m,p) = Add(n,p) <=> m = n’
+ >-- (
+ qexists_tac ‘Iff(Eq(N) o 
+                  Pa(Add(m o To1(N),id(N)),
+                     Add(n o To1(N),id(N))),
+                  Eq(N) o Pa(m,n) o To1(N))’
+ >-- rw[GSYM Iff_def,Pa_distr,p12_of_Pa,o_assoc,
+        IFF_def,GSYM Add_def] >>
+     once_rw[one_to_one_id] >> rw[idR,idL] >>
+     rw[Eq_property_TRUE,Add_def])>>
+ pop_assum strip_assume_tac >> 
+ qsuff_tac
+ ‘!p. P o p = TRUE’
+ >-- fs[ALL_property] >>
+ rw[IP_el] >> strip_tac
+ >-- arw[Add_O] >>
+ rpt strip_tac >> rfs[] >>
+ fs[Add_Suc,Suc_def,Suc_eq_eq])
+(form_goal
+ “!m:1->N n p. Add(m,p) = Add(n,p) <=> m = n”));
+
+val LESS_MONO_ADD_EQ = GSYM LESS_MONO_ADD
+                            |> store_as
+                            "LESS_MONO_ADD_EQ";
+
+val Sub_EQ_O = 
+ SUB_equal_0 |> rewr_rule[Sub_def]
+             |> store_as "Sub_EQ_O";
+
+val LESS_OR_EQ = prove_store("LESS_OR_EQ",
+e0
+(rpt strip_tac >> dimp_tac >> strip_tac 
+ >-- (drule Le_cases >> arw[]) 
+ >-- fs[Lt_def] >>
+ arw[Le_def,Sub_EQ_O] )
+(form_goal
+ “!m n:1->N. Le(m,n) <=> (Lt(m,n) | m = n)”));
+
+val LESS_EQ_MONO_ADD_EQ = prove_store
+("LESS_EQ_MONO_ADD_EQ",
+e0
+(rw[LESS_OR_EQ,LESS_MONO_ADD_EQ,EQ_MONO_ADD_EQ])
+(form_goal
+ “!m:1->N n p.Le(Add(m,p),Add(n,p)) <=> Le(m,n)”));
+ 
+val lej_property = prove_store("lej_property",
+e0
+(rw[lej_def,o_assoc,Pa_distr,p12_of_Pa,Add_def])
+(form_goal
+ “!a b c d. lej o Pa(Pa(a,b),Pa(c,d)) = TRUE <=> 
+ Le(Add(a,d),Add(b,c))”));
+
+val Le_refl = LE_refl |> rewr_rule[GSYM Le_def1]
+                      |> store_as "Le_refl";
+
+val lej_refl = prove_store("lej_refl",
+e0
+(strip_tac >> rw[lej_def] >>
+ qsspecl_then [‘p1(N,N) o ab’,‘p2(N,N) o ab’]
+ assume_tac Add_sym >> arw[Add_def] >>
+ rw[Le_refl])
+(form_goal
+ “!ab. lej o Pa(ab,ab) = TRUE”));
+
+val Le_Add = prove_store("Le_Add",
+e0
+(rpt strip_tac >> irule Le_trans >>
+ qexists_tac ‘Add(a,d)’ >> arw[LESS_EQ_MONO_ADD_EQ] >>
+ qsspecl_then [‘a’,‘b’] assume_tac Add_sym >>
+ arw[] >>
+ qsspecl_then [‘a’,‘d’] assume_tac Add_sym >>
+ arw[] >> arw[LESS_EQ_MONO_ADD_EQ])
+(form_goal
+ “!a:1->N b c d. Le(a,c) & Le(b,d) ==> Le(Add(a,b),Add(c,d))”));
+
+
+
+val lej_trans = prove_store("lej_trans",
+e0
+(rw[lej_def] >> rpt strip_tac >>
+ qsspecl_then  [‘a1’] assume_tac has_components >>
+ qsspecl_then  [‘a2’] assume_tac has_components >>
+ qsspecl_then  [‘a3’] assume_tac has_components >>
+ fs[] >> fs[] >> fs[p12_of_Pa,Add_def] >> 
+ qsuff_tac ‘Le(Add(Add(a,b''),Add(a',b')),
+               Add(Add(b,a''),Add(a',b')))’
+ >-- rw[LESS_EQ_MONO_ADD_EQ] >>
+ qsspecl_then [‘Add(a,b')’,‘Add(a',b'')’,
+               ‘Add(b,a')’,‘Add(b',a'')’]
+ assume_tac Le_Add >> rfs[] >>
+ qsuff_tac ‘Add(Add(a, b'), Add(a', b'')) = 
+ Add(Add(a, b''), Add(a', b')) & 
+ Add(Add(b, a'), Add(b', a'')) = 
+ Add(Add(b, a''), Add(a', b'))’
+ >-- (strip_tac >> fs[]) >> strip_tac >--
+ (once_rw[Add_sym] >>
+ qsspecl_then [‘a’,‘b''’] assume_tac Add_sym >> arw[] >>
+ rw[Add_assoc] >> 
+ qsspecl_then [‘Add(a',b')’,‘b''’] assume_tac Add_sym>>
+ arw[] >> rw[GSYM Add_assoc] >>
+ qsspecl_then [‘b'’,‘a’] assume_tac Add_sym >>
+ once_arw[] >> rw[Add_assoc] >>
+ qsspecl_then [‘b''’,‘a'’] assume_tac Add_sym >>
+ once_arw[] >> rw[]) >>
+ qsspecl_then [‘Add(b,a')’,‘Add(b',a'')’]
+ assume_tac Add_sym >> arw[] >>
+ qsspecl_then [‘b'’,‘a''’] assume_tac Add_sym >> arw[]>>
+ qsspecl_then [‘b’,‘a''’] assume_tac Add_sym >> arw[]>>
+ rw[GSYM Add_assoc] >>
+ qsuff_tac ‘Add(b', Add(b, a')) = Add(b, Add(a', b'))’
+ >-- (strip_tac >> arw[]) >>
+ qsspecl_then [‘a'’,‘b'’] assume_tac Add_sym >>
+ arw[] >>
+ rw[Add_assoc] >> 
+ qsspecl_then [‘b’,‘b'’] assume_tac Add_sym >> arw[])
+(form_goal
+ “!a1:1->N * N a2 a3. lej o Pa(a1,a2) = TRUE & lej o Pa(a2,a3) = TRUE ==> lej o Pa(a1,a3) = TRUE” ));
+
+
+val J1_x = prove_store("J1_x",
+e0
+(rw[lej_def,Addj_property,p12_of_Pa] >>
+ rw[Add_def] >> rpt strip_tac >>
+ qsuff_tac 
+ ‘Le(Add(Add(a, d), Add(e, f)), Add(Add(b, c), Add(e,f))) &
+  Add(Add(a, e), Add(d, f)) = Add(Add(a, d), Add(e, f)) & 
+  Add(Add(b, f), Add(c, e)) = Add(Add(b, c), Add(e, f))’
+ >-- (rpt strip_tac >> arw[]) >>
+ rpt strip_tac (* 3 *)
+ >-- arw[LESS_EQ_MONO_ADD_EQ]
+ >-- (rw[GSYM Add_assoc] >>
+      qsuff_tac ‘Add(e, Add(d, f)) = Add(d, Add(e, f))’ 
+      >-- (strip_tac >> arw[]) >>
+      rw[Add_assoc] >>
+      qsspecl_then [‘e’,‘d’] assume_tac Add_sym >> arw[]) >>
+ rw[GSYM Add_assoc] >>
+ qsuff_tac ‘Add(f, Add(c, e)) = Add(c, Add(e, f))’
+ >-- (strip_tac >> arw[]) >>
+ qsspecl_then [‘f’,‘Add(c,e)’] assume_tac Add_sym >> arw[] >>
+ rw[Add_assoc] )
+(form_goal
+ “!a b c d e f. 
+  lej o Pa(Pa(a,b),Pa(c,d)) = TRUE ==>
+  lej o Pa(Addj(Pa(a,b),Pa(e,f)),
+           Addj(Pa(c,d),Pa(e,f))) = TRUE”));
+
+
+
+val J2_iv = prove_store("J2_iv",
+e0
+(once_rw[lej_def] >> once_rw[ZR_def] >>
+ rw[Fst_Snd_Pa] >>
+ rw[p12_of_Pa] >> once_rw[Add_def] >>
+ rpt strip_tac >> 
+ qsuff_tac 
+ ‘(Le(Add(a, d), Add(b, c)) <=> 
+  Le(Add(Add(a,d),Add(b',d')), Add(Add(b,c),Add(b',d')))) &
+  (Le(Add(Add(a,d),Add(b',d')), Add(Add(b,c),Add(b',d'))) <=> 
+  Le(Add(Add(a',d'),Add(b,d)), Add(Add(b',c'),Add(b,d)))) & 
+  (Le(Add(Add(a',d'),Add(b,d)), Add(Add(b',c'),Add(b,d))) <=> 
+ Le(Add(a',d'), Add(b',c')))’
+ >-- (rpt strip_tac >> arw[]) >> rpt strip_tac (* 3 *)
+ >-- rw[LESS_EQ_MONO_ADD_EQ] 
+ >-- (qsuff_tac ‘Add(Add(a, d), Add(b', d')) = 
+                Add(Add(a', d'), Add(b, d)) & 
+                Add(Add(b, c), Add(b', d')) = 
+                Add(Add(b', c'), Add(b, d))’
+     >-- (strip_tac >> arw[]) >> strip_tac (* 2 *)
+     >-- (qsspecl_then [‘Add(b',d')’,‘Add(a,d)’] 
+          assume_tac $ GSYM Add_sym >> arw[] >>
+          qsspecl_then [‘d'’,‘b'’] assume_tac $ GSYM Add_sym >> arw[] >>
+          rw[Add_assoc] >>
+          qsuff_tac ‘Add(Add(d', b'), a) = 
+                     Add(Add(a', d'), b)’
+          >-- (strip_tac >> arw[]) >>
+          qsspecl_then [‘d'’,‘a'’] assume_tac $GSYM Add_sym >> arw[] >>
+          rw[GSYM Add_assoc] >> 
+          qsspecl_then [‘a’,‘b'’] assume_tac $GSYM Add_sym >> arw[] >>
+          qsspecl_then [‘a'’,‘b’] assume_tac  Add_sym >> arw[]) >>
+     qsspecl_then [‘Add(b',d')’,‘Add(b,c)’] assume_tac$GSYM Add_sym >>
+     arw[] >> 
+     qsspecl_then [‘c’,‘b’] assume_tac $GSYM Add_sym >> arw[] >>
+     qsspecl_then [‘d’,‘b’] assume_tac $GSYM Add_sym >> arw[] >>
+     rw[Add_assoc] >>
+     qsuff_tac ‘Add(Add(b', d'), c) = Add(Add(b', c'), d)’ 
+     >-- (strip_tac >> arw[]) >>
+     rw[GSYM Add_assoc] >>
+     qsspecl_then [‘c’,‘d'’] assume_tac $GSYM Add_sym >> arw[] >>
+  qsspecl_then [‘c'’,‘d’] assume_tac $GSYM Add_sym >> arw[]) >>
+ rw[LESS_EQ_MONO_ADD_EQ] 
+ )
+(form_goal “!a b c d a' b' c' d'. 
+ ZR(Pa(a,b),Pa(a',b')) &
+ ZR(Pa(c,d),Pa(c',d')) ==> 
+(lej o Pa(Pa(a,b),Pa(c,d)) = TRUE <=>
+lej o Pa(Pa(a',b'),Pa(c',d')) = TRUE)”));
+
+val LEz_ex = prove_store("LEz_ex",
+e0
+(qexists_tac ‘lej o Pa(REP o p1(Z,Z),REP o p2(Z,Z))’ >>
+ rw[o_assoc,Pa_distr,p12_of_Pa,rep_def])
+(form_goal
+ “?lez. !z1 z2. lez o Pa(z1,z2) = TRUE <=> 
+ lej o Pa(rep(z1),rep(z2)) = TRUE”));
+
+val LEz_def = LEz_ex |> ex2fsym0 "LEz" []
+                     |> store_as "LEz_def";
+
+val LEz_refl = prove_store("LEz_refl",
+e0
+(rw[LEz_def,lej_refl])
+(form_goal
+ “!z. LEz o Pa(z,z) = TRUE”));
+
+val LEz_trans = prove_store("LEz_trans",
+e0
+(assume_tac lej_trans >>
+ rw[LEz_def] >> rpt strip_tac >>
+ qsspecl_then [‘rep(a1)’] assume_tac has_components >> 
+ qsspecl_then [‘rep(a2)’] assume_tac has_components >>
+ qsspecl_then [‘rep(a3)’] assume_tac has_components >>
+ pop_assum_list (map_every strip_assume_tac) >>
+ arw[] >> first_x_assum irule >> rfs[] >>
+ qexists_tac ‘Pa(a',b')’ >> arw[])
+(form_goal
+ “!a1:1->Z a2 a3. LEz o Pa(a1,a2) = TRUE & LEz o Pa(a2,a3) = TRUE ==> 
+ LEz o Pa(a1,a3) = TRUE”));
+
+val Suc_NONZERO = prove_store("Suc_NONZERO",
+e0
+(rw[O_xor_SUC] >> 
+ strip_tac >> qexists_tac ‘n’ >> rw[Suc_def])
+(form_goal
+ “!n. ~(Suc(n) =O)”));
+
+val WOP' = prove_store("WOP'",
+e0
+(assume_tac WOP >>
+ rw[Le_def1] >> rpt strip_tac >> first_x_assum irule >>
+ ccontra_tac >>
+ fs[False2FALSE,TRUE_ne_FALSE])
+(form_goal
+ “!P:N -> 1+1 a.
+        P o a = TRUE ==>
+        ?(l : ar(1, N)).
+          P o l = TRUE &
+          !n. P o n = TRUE ==> Le(l,n)”));
+
+val Suc_NEQ = prove_store("Suc_NEQ",
+e0
+(qby_tac
+ ‘?P. !a. P o a = TRUE <=> (a = Suc(a))’
+ >-- (qexists_tac ‘Eq(N) o Pa(id(N),SUC)’ >>
+      rw[o_assoc,Pa_distr,Eq_property_TRUE,
+       idL,Suc_def]) >>
+ pop_assum (strip_assume_tac o GSYM) >>
+ strip_tac >> ccontra_tac >>
+ rfs[] >> drule WOP' >>
+ pop_assum strip_assume_tac >>
+ cases_on “l = O” >--
+ (last_x_assum (assume_tac o GSYM) >> fs[GSYM Suc_NONZERO]) >>
+ fs[O_xor_SUC] >>
+ last_x_assum (assume_tac o GSYM) >> fs[Suc_eq_eq,Suc_def] >>
+ first_x_assum drule >> 
+ drule $ iffRL Lt_Suc_Le >> fs[Lt_def])
+(form_goal “!a:1->N. ~(a = Suc(a))”));
+
+val Sub_Suc = SUB_SUC |> rewr_rule[Sub_def,Suc_def,Pre_def]
+                      |> store_as "Sub_Suc";
+
+val Pre_O = PRE_def |> conjE1 |> conjE1 |> rewr_rule[Pre_def]
+                    |> store_as "Pre_O";
+
+val Lt_Suc = prove_store("Lt_Suc",
+e0
+(rw[Lt_def,Le_def,Sub_Suc,Suc_NEQ,Sub_EQ_O,Pre_O])
+(form_goal “!a:1->N. Lt(a,Suc(a))”));
+
+val O_xor_Suc = O_xor_SUC |> rewr_rule[Suc_def]
+                          |> store_as "O_xor_Suc";
+
+val Add_Suc_Lt = prove_store("Add_Suc_Lt",
+e0
+(strip_tac >>
+ qby_tac ‘?P. !b. Lt(a,Add(a,Suc(b))) <=> P o b = TRUE’
+ >-- (qexists_tac 
+      ‘Char(LT) o Pa(a o To1(N), ADD o Pa(a o To1(N),SUC))’ >>
+      rw[GSYM Lt_def1,o_assoc,Pa_distr,Suc_def] >>
+      once_rw[one_to_one_id] >> rw[idR,Add_def]) >>
+ pop_assum strip_assume_tac >> arw[] >>
+ rw[IP_el] >> pop_assum (assume_tac o GSYM) >> arw[] >> strip_tac>--
+(rw[Lt_def,Le_def,Add_Suc,Add_O,Sub_Suc,Pre_O,O_xor_Suc,
+        Suc_NEQ,Pre_O,Sub_EQ_O]) >>
+ rpt strip_tac >> rw[Add_Suc] >> rw[Lt_Suc_Le] >>
+ rw[GSYM Add_Suc] >> fs[Lt_def,Suc_def]
+ )
+(form_goal
+ “!a:1->N b. Lt(a,Add(a,Suc(b)))”));
+
+
+val Lt_trans = prove_store("Lt_trans",
+e0
+(rw[Lt_def] >>
+ assume_tac Le_trans >> rpt strip_tac >--
+ (first_x_assum irule >> qexists_tac ‘a2’ >> arw[]) >>
+ qby_tac ‘(?p1. Add(a1,Suc(p1)) = a2) & 
+          ?p2. Add(a2,Suc(p2)) = a3’ >-- 
+ (drule Le_Add_ex >> rev_drule Le_Add_ex >> fs[] >>
+ qby_tac ‘~(p = O)’
+ >-- (ccontra_tac >> fs[Add_O2]) >>
+ qby_tac ‘~(p' = O)’
+ >-- ccontra_tac >> fs[Add_O2] >>
+ fs[O_xor_Suc] >> strip_tac 
+ >-- (qexists_tac ‘n0'’ >> arw[] >> once_rw[Add_sym] >> fs[]) >>
+ (qexists_tac ‘n0’ >> arw[] >> once_rw[Add_sym] >> fs[])) >>
+ cheat >>
+ pop_assum (strip_assume_tac o GSYM) >>
+ fs[] >> rw[GSYM Add_assoc] >> once_rw[Add_Suc] >>
+ assume_tac Add_Suc_Lt >> fs[Lt_def])
+(form_goal “!a1:1->N a2 a3. Lt(a1,a2) & Lt(a2,a3) ==> Lt(a1,a3)”));
+
+
+(*TODO: delete LE_cases_iff*)
+
+val Le_asym = prove_store("Le_asym",
+e0
+(rpt strip_tac >> drule Le_cases >> pop_assum strip_assume_tac >>
+ arw[] >> rev_drule Le_cases >> pop_assum strip_assume_tac >> arw[] >>
+ qby_tac ‘Lt(a,a)’ 
+ >-- (irule Lt_trans >> qexists_tac ‘b’ >> arw[]) >>
+ fs[Lt_def])
+(form_goal
+ “!a:1->N b. Le(a,b) & Le(b,a) ==> a = b”));
+
+val LEz_asym = prove_store("LEz_asym",
+e0
+(rw[LEz_def] >> strip_tac >> strip_tac >>
+ qsspecl_then [‘rep(a)’] assume_tac has_components >> 
+ qsspecl_then [‘rep(b)’] assume_tac has_components >>
+ pop_assum_list (map_every strip_assume_tac) >> arw[] >>
+ rw[lej_def] >> rw[p12_of_Pa,Add_def] >> strip_tac >>
+ once_rw[z_eq_cond] >>
+ qexistsl_tac [‘Pa(a'',b'')’,‘Pa(a',b')’] >>
+ rw[ZR_def] >> rw[Fst_Snd_Pa] >> rpt strip_tac (* 3 *)
+ >-- (pop_assum_list (map_every (assume_tac o GSYM)) >>
+      arw[rep_asz])
+ >-- (pop_assum_list (map_every (assume_tac o GSYM)) >>
+      arw[rep_asz]) >>
+ irule Le_asym  >> 
+ qsspecl_then [‘a''’,‘b'’] assume_tac $GSYM Add_sym >>fs[] >>
+ qsspecl_then [‘a'’,‘b''’] assume_tac $GSYM Add_sym >> fs[])
+(form_goal
+ “!a b. LEz o Pa(a,b) = TRUE & LEz o Pa(b,a) = TRUE ==> a = b”));
+
+
+
+val LEz_total = prove_store("LEz_total",
+e0
+(rw[LEz_def,lej_def] >> rpt strip_tac >>
+ qsspecl_then [‘rep(a)’] assume_tac has_components >> 
+ qsspecl_then [‘rep(b)’] assume_tac has_components >>
+ pop_assum_list (map_every strip_assume_tac) >> 
+ arw[p12_of_Pa] >>
+ qsspecl_then [‘a'’,‘b''’] assume_tac $GSYM Add_sym >> arw[] >>
+ qsspecl_then [‘a''’,‘b'’] assume_tac $GSYM Add_sym >> arw[] >>
+ arw[Add_def] >> rw[Le_def1] >>
+ rw[LESS_EQ_cases] )
+(form_goal “!a:1->Z b. LEz o Pa(a,b) = TRUE | LEz o Pa(b,a) = TRUE”));
+
+
+val Z = mk_fun "Z" []
+
+val _ = new_pred "Lez" [("z1",ar_sort (mk_ob "X") Z),
+                        ("z2",ar_sort (mk_ob "X") Z)]
+
+val Lez_def0 = store_ax("Lez_def0",
+“!X z1:X->Z z2.Lez(z1,z2) <=> LEz o Pa(z1,z2) = True(X)”);
+
+val Lez_def = Lez_def0 |> allE (rastt "1")
+                       |> rewr_rule[True1TRUE]
+                       |> store_as "Lez_def";
+
+
+val J2_iv' = prove_store("J2_iv'",
+e0
+(rpt strip_tac >> 
+ qsspecl_then [‘ab’] assume_tac has_components >>
+ qsspecl_then [‘ab'’] assume_tac has_components >>
+ qsspecl_then [‘cd’] assume_tac has_components >>
+ qsspecl_then [‘cd'’] assume_tac has_components >>
+ pop_assum_list (map_every strip_assume_tac) >> rfs[] >>
+ irule J2_iv >> arw[])  
+(form_goal
+ “!ab cd ab' cd'. ZR(ab,ab') & ZR(cd,cd') ==> 
+ (lej o Pa(ab,cd) = TRUE <=> lej o Pa(ab',cd') = TRUE)”));
+
+
+
+
+
+val Z2_x = prove_store("Z2_x",
+e0
+(rw[Lez_def,Addz_eqn',Addj_property,LEz_def] >>
+ rpt strip_tac >>
+ qsuff_tac 
+ ‘lej o Pa(Pa(a, b),Pa(c, d)) = TRUE ==> 
+  lej o Pa (Pa(Add(a, e), Add(b, f)),
+            Pa(Add(c, e), Add(d, f))) = TRUE’ >--
+ (rpt strip_tac >>
+ qby_tac ‘lej o Pa(Pa(a, b), Pa(c, d)) = TRUE’
+ >-- (irule $ iffLR J2_iv' >>
+      qexistsl_tac 
+      [‘rep(asz(Pa(a, b)))’,‘rep(asz(Pa(c, d)))’]>>
+      arw[] >> rw[GSYM rep_rel_all]) >>
+ first_x_assum drule >> 
+ irule $ iffLR J2_iv' >>
+ qexistsl_tac
+ [‘Pa(Add(a, e), Add(b, f))’,‘Pa(Add(c, e), Add(d, f))’] >>
+ arw[] >> once_rw[ZR_sym] >> rw[GSYM rep_rel_all]) >>
+ pop_assum (K all_tac) >>
+ rw[lej_property] >> rpt strip_tac >>
+ qsspecl_then [‘Add(d,f)’,‘Add(a,e)’] assume_tac $ GSYM Add_sym >>
+ arw[] >> rw[Add_assoc] >> rw[LESS_EQ_MONO_ADD_EQ] >>
+ once_rw[Add_sym] >> rw[Add_assoc] >>
+ rw[LESS_EQ_MONO_ADD_EQ] >> 
+ qsspecl_then [‘c’,‘b’] assume_tac$ GSYM Add_sym >> fs[]
+ )
+(form_goal “!a:1->N b c d e f.Lez(asz(Pa(a,b)),asz(Pa(c,d))) ==>
+            Lez(Addz(asz(Pa(a,b)),asz(Pa(e,f))),
+                Addz(asz(Pa(c,d)),asz(Pa(e,f))))”));
+
+
+(*
+val lej_ex = prove_store("lej_ex",
+e0
+()
+(form_goal
+ “?lej. !a:1-> N b c d. 
+  lej o Pa(Pa(a,b),Pa(c,d)) = TRUE <=> 
+  Le(Add(a,d),Add(b,c))”));
+*)
+
+
+(*
+rastt "Ev(X,2) o (f :1-> X * Pow(X))"
+
+
+
+should be same 
+rastt "Ev(X,2) o f: 1-> X * Exp(X,2)"
+
+otherwise cannot unify 
+
+so the subst from Pow(X) into Exp(X,2) must be done before unification
+
+two dictionaries 
+
+Exp(X,2) <> Pow(X)
+
+("Pow",([("X",ob)],Exp(X,2) as a ast))
+
+
+then use an inst_ast version of inst_term 
+
+*)
+
+(*
+
+fun subst_ast a1 a2 ast = 
+case ast of 
+    aId(a) => if aId(a) = a1 then a2 else ast
+   | aApp(str,astl) => 
+     if ast = a1 then a2 else
+     aApp(str,List.map (subst_ast a1 a2) astl)
+   | aInfix(ast1,str,ast2) =>
+    aInfix(subst_ast a1 a2 ast1,str,subst_ast a1 a2 ast2)
+   | aBinder(str,ns,b) =>
+     aBinder(str,subst_ast a1 a2 ns,subst_ast a1 a2 b)
+
+
+val abbrevs0 = [("Exp",["X",ob_sort])]
+
+*)
+
+
+(*cannot be like fsyms psyms dict, should it be a dictionary at all?
+
+thought about using something like ("Exp",([old arguments],[new_arguments]), and strings as key, but then the pp need another dictionary, seems weird.)
+*)
+
+
+(*fun subst_abbr ast = 
+
+the obvious thing is to write a code that search if there is any occurrence of each abbreved term and replace them.
+
+but then need to look through the dictionary and find out each occurence of any abbreved term.
+
+Any better way to write this?
+
+
+*)
+
+
+
+
+
